Ad skeleton danfy function to in

src/dafny/smart/Deposit.dfy
@@ -36,7 +36,19 @@ module DepositTree {
 
             case Node(v, lc, rc, _, _) => v == hash(lc.v, rc.v)
     }
+        function method diff(a: int, b : int) : int 
+    {
+        a - b
+    }
 
+        function power2(n : nat): nat 
+        ensures power2(n) >= 1
+        ensures n >= 1 ==> power2(n) >= 2 
+
+        decreases n
+    {
+        if n == 0 then 1 else 2 * power2(n - 1)
+    }
     /**
      *  Incremental algorithm.
      */
@@ -49,6 +61,46 @@ module DepositTree {
         *         zerohashes[i+1] = hash(zerohashes[i], zerohashes[i])
         *         i += 1
         */
+
+        ghost var root: Tree<int>
+        const TREE_HEIGHT: nat
+        var zerohashes: array<int>
+
+        var deposit_count: int
+
+        var branch: array<int>
+
+        predicate Valid()
+        reads this
+            {
+                deposit_count < power2(TREE_HEIGHT) - 1 &&
+                branch.Length == TREE_HEIGHT == zerohashes.Length &&
+                TREE_HEIGHT == height(root) 
+            }
+
+        method initializeZeroHashes()
+        requires Valid()
+        requires TREE_HEIGHT > 1
+        modifies zerohashes
+        requires zerohashes.Length == TREE_HEIGHT
+        requires forall i :: 0 <= i < zerohashes.Length ==> zerohashes[i] == 0
+        ensures Valid()
+        ensures forall i :: 0 <= i < zerohashes.Length - 1 ==> zerohashes[i+1] == diff(zerohashes[i],zerohashes[i])
+        {
+
+            var x := 0;
+
+            while x != TREE_HEIGHT - 1
+                invariant 0 <= x < TREE_HEIGHT
+                invariant forall i :: 0 <= i < x ==> zerohashes[i+1] == diff(zerohashes[i],zerohashes[i])
+                invariant forall i :: x < i < zerohashes.Length ==> zerohashes[i] == 0
+                decreases TREE_HEIGHT - x 
+                {
+                    zerohashes[x+1] := diff(zerohashes[x],zerohashes[x]);
+                    x := x + 1;
+                }
+
+        }
 
         /*
         * fun deposit(value: int) -> unit:
@@ -65,8 +117,35 @@ module DepositTree {
         *     branch[i] = value
         */
 
+        method deposit(value: int) returns (t: int)
+            requires Valid()
+            modifies this
+            modifies branch
+            ensures Valid()
+            {
+
+                var n := 0;
+                deposit_count := deposit_count + 1;
+                var value1 := value;
+                var size;
+                while n != TREE_HEIGHT
+                    invariant 0 <= n <= TREE_HEIGHT 
+                    invariant deposit_count < power2(TREE_HEIGHT) 
+                    decreases TREE_HEIGHT - n 
+                    {
+                        if deposit_count % 2 == 1 {
+                            break;
+                        }
+                        value1 := diff(branch[n], value);
+                        size := deposit_count / 2;
+                        n := n + 1;
+                    }
+                    assert TREE_HEIGHT == branch.Length;
+                    branch[n] := value;
+            }
+
         /*
-        * fun get_deposit_root() -> int:
+        * fun __deposit_root() -> int:
         *     root: int = 0
         *     size: int = deposit_count
         *     h: int = 0
@@ -79,6 +158,30 @@ module DepositTree {
         *         h += 1
         *     return root
         */
+
+        method deposit_root() returns (r: int)
+            requires Valid()
+            ensures Valid()
+            {
+                
+                var n := 0;
+                var size := 0;
+                while n != TREE_HEIGHT
+                    invariant 0 <= n <= TREE_HEIGHT
+                    decreases TREE_HEIGHT - n
+                    {
+                        if deposit_count % 2 == 1 {
+                            r := diff(branch[n], r);
+                        }else {
+                            r := diff(r, zerohashes[n]);
+                        }
+                        size := size / 2;
+                        n := n + 1;
+                        
+                    }
+                    assert 
+                    return r;
+            }
 
 } 
    
